Certifying passes (#86)
* Certifying (proof-generation) expansion of match branches
* Certifying inlining
* Introduce the certifying pipeline: apply transforms at the template coq level and generate proofs after all template passes; 
* Integrated the pipeline into Liquidity and Elm extraction.

Co-authored-by: Jakob Botsch Nielsen <Jakob.botsch.nielsen@gmail.com>

extraction/theories/CertifyingEta.v
@@ -5,9 +5,12 @@
     Coq's conversion, the proof is essentially [eq_refl].
     All dependencies are also expanded.*)
 
-From Coq Require Import List PeanoNat Bool String.
-From MetaCoq.Template Require Import Kernames All.
-From ConCert.Extraction Require Import Erasure Optimize Common ResultMonad Extraction.
+From Coq Require Import List PeanoNat Bool Ascii String.
+From MetaCoq.Template Require Import Kernames All Ast.
+From ConCert.Extraction Require Import
+     Erasure Optimize Common ResultMonad Extraction Certifying.
+From ConCert.Utils Require StringExtra.
+
 Open Scope string.
 Open Scope nat.
 
@@ -79,6 +82,17 @@ Definition eta_const (kn : kername) (u : Instance.t) (args : list term) : term :
   | None => mkApps (tConst kn u) args
   end.
 
+Fixpoint eta_branch (ar : nat) (body : term) : term :=
+  match ar with
+  | 0 => body
+  | S ar =>
+    match body with
+    | tLambda na ty body => tLambda na ty (eta_branch ar body)
+    | _ => tLambda (mkBindAnn nAnon Relevant) hole (eta_branch ar (mkApp (lift0 1 body) (tRel 0)))
+    end
+  end.
+
+
 Definition get_ind_info (ind : inductive) : option ind_info :=
    match lookup_env Σ ind.(inductive_mind) with
       | Some (InductiveDecl mib) =>
@@ -108,11 +122,12 @@ Fixpoint eta_expand (t : term) : term :=
   | tLambda na ty body => tLambda na ty (eta_expand body)
   | tLetIn na val ty body => tLetIn na (eta_expand val) ty (eta_expand body)
   | tCase p ty disc brs =>
-    tCase p ty (eta_expand disc) (map (on_snd eta_expand) brs)
+    let on_branch '(ar, t) := (ar, eta_branch ar (eta_expand t)) in
+    tCase p ty (eta_expand disc) (map on_branch brs)
   | tProj p t => tProj p (eta_expand t)
   | tFix def i => tFix (map (map_def id eta_expand) def) i
   | tCoFix def i => tCoFix (map (map_def id eta_expand) def) i
-  (* NOTE: we know that constructros and constants are not applied at this point,
+  (* NOTE: we know that constructors and constants are not applied at this point,
      since applications are captured by the previous cases *)
   | tConstruct ind c u =>
     match get_ind_info ind with
@@ -150,71 +165,6 @@ Fixpoint get_eta_info (Σ : global_env) (ds : dearg_set) : ctors_info * constans
   | [] => ([],[])
   end.
 
-Fixpoint change_modpath (mpath : modpath) (ignore : kername -> bool) (t : term) : term :=
-  match t with
-  | tRel n => t
-  | tVar id => t
-  | tSort s => t
-  | tEvar ev args => tEvar ev (map (change_modpath mpath ignore) args)
-  | tCast t kind v => tCast (change_modpath mpath ignore t) kind (change_modpath mpath ignore v)
-  | tProd na ty body => tProd na (change_modpath mpath ignore ty) (change_modpath mpath ignore body)
-  | tLambda na ty body => tLambda na (change_modpath mpath ignore ty) (change_modpath mpath ignore body)
-  | tLetIn na def def_ty body =>
-    tLetIn na (change_modpath mpath ignore def) (change_modpath mpath ignore def_ty) (change_modpath mpath ignore body)
-  | tApp f args => tApp (change_modpath mpath ignore f) (map (change_modpath mpath ignore) args)
-  | tConst kn u => if ignore kn then t
-                  else tConst (mpath, kn.2 ++ "_expanded") u
-  | tInd ind u => t
-  | tConstruct ind idx u => t
-  | tCase ind_and_nbparams type_info discr branches =>
-    tCase ind_and_nbparams (change_modpath mpath ignore type_info)
-          (change_modpath mpath ignore discr) (map (on_snd (change_modpath mpath ignore)) branches)
-  | tProj proj t => tProj proj (change_modpath mpath ignore t)
-  | tFix mfix idx => tFix (map (map_def (change_modpath mpath ignore) (change_modpath mpath ignore)) mfix) idx
-  | tCoFix mfix idx => tCoFix (map (map_def (change_modpath mpath ignore) (change_modpath mpath ignore)) mfix) idx
-  | tInt _ => t
-  | tFloat _ => t
-  end.
-
-Definition generate_proof (Σ1 Σ2 : global_env) (kn1 kn2 : kername) : TemplateMonad (term × term × term × term) :=
-  match lookup_env Σ1 kn1, lookup_env Σ2 kn2  with
-  | Some (ConstantDecl cb1), Some (ConstantDecl cb2) =>
-    match cb1.(cst_body), cb2.(cst_body) with
-    | Some _, Some exp_body =>
-      let ty := cb1.(cst_type) in
-      let proof_ty :=
-          tApp (tInd
-                  {| inductive_mind := (MPfile ["Logic"; "Init"; "Coq"], "eq");
-                     inductive_ind := 0 |} [])
-               [ty; tConst kn1 []; tConst kn2 []] in
-      let proof_body := tApp (tConstruct
-                          {| inductive_mind := (MPfile ["Logic"; "Init"; "Coq"], "eq");
-                             inductive_ind := 0 |} 0 [])
-                       [ty;tConst kn1 []] in
-      ret (cb1.(cst_type), (exp_body, (proof_ty, proof_body)))
-    | _,_ => tmFail "No body"
-    end
-  | None, _ => tmFail ("Not found: " ++ kn1.2)
-  | _, None => tmFail ("Not found: " ++ kn2.2)
-  | _,_ => tmFail "Not a constant"
-  end.
-
-Definition gen_proof_prog (Σ1 Σ2 : global_env) (kn1 kn2 : kername) : TemplateMonad unit :=
-  '(exp_ty, (exp_t, (p_ty, p_t))) <- generate_proof Σ1 Σ2 kn1 kn2 ;;
-  tmBind (tmUnquoteTyped Type exp_ty)
-         (fun A => ucst <- tmUnquoteTyped A exp_t ;;
-                 tmDefinition kn2.2 ucst;;
-            tmBind (tmUnquoteTyped Type p_ty)
-                   (fun B =>
-                      uproof <- tmUnquoteTyped B p_t ;;
-                      tmDefinition (kn2.2++"_correct") uproof ;;
-                      tmPrint B)).
-
-Definition contains_global_env (Σ : global_env) (kn : kername) :=
-  match lookup_env Σ kn with
-  | Some v => true
-  | None => false
-  end.
 
 Definition restrict_env (Σ : global_env) (kns : list kername) : global_env :=
   filter (fun '(kn, _) => match find (eq_kername kn) kns with
@@ -222,28 +172,13 @@ Definition restrict_env (Σ : global_env) (kns : list kername) : global_env :=
                        | None => false
                        end) Σ.
 
-Fixpoint map_constants_global_env (k : kername -> kername) (f : constant_body -> constant_body) (Σ : global_env) : global_env :=
-  match Σ with
-  | [] => []
-  | (kn, ConstantDecl cb) :: Σ' => (k kn, ConstantDecl (f cb)) :: map_constants_global_env k f Σ'
-  | gd :: Σ' => gd :: map_constants_global_env k f Σ'
-  end.
-
-Definition add_suffix_global_env (mpath : modpath) (ignore : kername -> bool) (Σ : global_env) :=
-  map_constants_global_env
-    (fun kn => (mpath,kn.2 ++ "_expanded"))
-    (fun cb => {| cst_type := cb.(cst_type);
-               cst_body := b <- cb.(cst_body);;
-                           Some (change_modpath mpath ignore b);
-                cst_universes := cb.(cst_universes) |}) Σ.
-
 Definition eta_global_env
            (trim_consts trim_inds : bool)
-           (Σ : global_env) (seeds : KernameSet.t) (ignore : kername -> bool) :=
+           (Σ : global_env) (seeds : KernameSet.t) (erasure_ignore : kername -> bool) :=
   let Σe :=
       erase_global_decls_deps_recursive
         (TemplateToPCUIC.trans_global_decls Σ) (assume_env_wellformed _)
-        seeds ignore in
+        seeds erasure_ignore in
   let (const_masks, ind_masks) := analyze_env Σe in
   let const_masks := (if trim_consts then trim_const_masks else id) const_masks in
   let ind_masks := (if trim_inds then trim_ind_masks else id) ind_masks in
@@ -258,38 +193,25 @@ Definition eta_global_env
       end in
   let Σ' := restrict_env Σ (map (fun '(kn, _, _) => kn) Σe) in
   map_constants_global_env id f Σ'.
-
-Definition is_none {A} (o : option A) :=
-  match o with
-  | Some _ => false
-  | None => true
-  end.
-
-Definition gen_expanded_const_and_proof (Σ : global_env) (mpath : modpath) (ignore : kername -> bool)  : TemplateMonad unit :=
-  let Σdecls := filter (fun '(kn,gd) => match gd with
-                                    | ConstantDecl cb => negb (is_none cb.(cst_body))
-                                    | _ => false
-                                     end) Σ in
-  Σdecls' <- tmEval lazy (add_suffix_global_env mpath ignore Σdecls) ;;
-  monad_iter (fun kn1 => gen_proof_prog Σ Σdecls' kn1 (mpath,kn1.2 ++ "_expanded"))
-             (List.rev (map fst Σdecls)).
-
 Definition eta_global_env_template
            (trim_consts trim_inds : bool)
            (mpath : modpath)
            (Σ : global_env)
-           (seeds : KernameSet.t) (ignore : kername -> bool)
-           (cst_name_ignore : kername -> bool) : TemplateMonad global_env :=
-  Σext <- tmEval lazy (eta_global_env trim_consts trim_inds Σ seeds ignore);;
-  gen_expanded_const_and_proof Σext mpath cst_name_ignore;;
+           (seeds : KernameSet.t) (erasure_ignore : kername -> bool)
+  : TemplateMonad global_env :=
+  let suffix := "_expanded" in
+  Σext <- tmEval lazy (eta_global_env trim_consts trim_inds Σ seeds erasure_ignore);;
+  gen_defs_and_proofs Σ Σext mpath suffix seeds;;
   ret Σext.
 
-Definition eta_expand_def {A} (trim_inds trim_consts : bool) (mpath : modpath) (cst_name_ignore : kername -> bool) (def : A) : TemplateMonad _ :=
+(* Mainly for testing purposes *)
+Definition eta_expand_def {A} (trim_inds trim_consts : bool) (def : A) : TemplateMonad _ :=
+  cur_mod <- tmCurrentModPath tt;;
   p <- tmQuoteRecTransp def false ;;
   kn <- extract_def_name def ;;
   eta_global_env_template
-    trim_inds trim_consts mpath p.1
-    (KernameSet.singleton kn) (fun _ => false) cst_name_ignore.
+    trim_inds trim_consts cur_mod p.1
+    (KernameSet.singleton kn) (fun _ => false).
 
 Module Examples.
 
@@ -300,30 +222,16 @@ Module Examples.
   End Ex1.
   MetaCoq Quote Recursively Definition p_app_pair_syn := Ex1.partial_app_pair.
 
-  Definition anchor := fun x : nat => x.
-  Definition CURRENT_MODULE := Eval compute in <%% anchor %%>.1.
-
   Definition modpath_eq_dec (mp1 mp2 : modpath) : {mp1 = mp2} + {mp1 <> mp2}.
     repeat decide equality.
   Defined.
 
-  Definition eq_modpath (mp1 mp2 : modpath) : bool :=
-    match modpath_eq_dec mp1 mp2 with
-    | left _ => true
-    | right _ => false
-    end.
-
-  Definition only_from_module_of (kn_base : kername) :=
-    fun (kn : kername) => negb (eq_modpath kn_base.1 kn.1).
-
   Module Test1.
-    Definition anchor := fun x : nat => x.
-    Definition CURRENT_MODULE := Eval compute in <%% anchor %%>.1.
-    MetaCoq Run (eta_global_env_template
-                   false false CURRENT_MODULE
+    MetaCoq Run (cur_mod <- tmCurrentModPath tt;;
+                 eta_global_env_template
+                   false false cur_mod
                    p_app_pair_syn.1
                    (KernameSet.singleton <%% Ex1.partial_app_pair %%>)
-                   (fun _ => false)
                    (fun _ => false)).
   End Test1.
 
@@ -340,15 +248,13 @@ Module Examples.
   (** Expands the dependencies and adds the corresponding definitions *)
   MetaCoq Run (eta_expand_def
                  true true
-                 CURRENT_MODULE
-                 (only_from_module_of <%% Ex2.partial_app2 %%>)
                  Ex2.partial_app2).
 
   (** [partial_app2_expanded] is defined in terms of [partial_app1_expanded] *)
-  Print partial_app2_expanded.
-  (* partial_app2_expanded =
-  let f := fun H H0 : Type => partial_app1_expanded H H0 in f bool true
-       : bool -> true -> MyInd bool true bool
+  Print ConCert_Extraction_CertifyingEta_Examples_Ex2_partial_app2_expanded.
+  (* ConCert_Extraction_CertifyingEta_Examples_Ex2_partial_app2_expanded =
+  let f := fun A B : Type => ConCert_Extraction_CertifyingEta_Examples_Ex2_partial_app1_expanded A B in f bool true
+     : bool -> true -> MyInd bool true bool
    *)
 
   Inductive MyInd1 (A B C : Type) :=
@@ -358,11 +264,7 @@ Module Examples.
   Definition partial_app3 A B n m :=
     let f := miCtor1 A in f B bool n m I.
 
-  MetaCoq Run (eta_expand_def
-                 true true
-                 CURRENT_MODULE
-                 (only_from_module_of <%% partial_app3 %%>)
-                 partial_app3).
+  MetaCoq Run (eta_expand_def true true partial_app3).
 
   Module Ex3.
   Definition inc_balance (st :  nat × nat) (new_balance : nat)
@@ -371,17 +273,14 @@ Module Examples.
 
   Definition partial_inc_balance st i := inc_balance st i.
   End Ex3.
-  MetaCoq Run (p <- tmQuoteRecTransp Ex3.partial_inc_balance false ;;
+  MetaCoq Run (cur_mod <- tmCurrentModPath tt;;
+               p <- tmQuoteRecTransp Ex3.partial_inc_balance false ;;
                eta_global_env_template
                  true true
-                 CURRENT_MODULE
+                 cur_mod
                  p.1
-                 (KernameSet.union
-                    (KernameSet.singleton <%% Ex3.inc_balance %%>)
-                    (KernameSet.singleton <%% Ex3.partial_inc_balance %%>))
-                 (fun kn => eq_kername kn <%% Ex3.inc_balance %%> ||
-                            eq_kername kn <%% Ex3.partial_inc_balance %%>)
-                 (only_from_module_of <%% Ex3.partial_inc_balance %%>)
+                 (KernameSet.singleton <%% Ex3.partial_inc_balance %%>)
+                 (fun _ => false)
               ).
 
   Module Ex4.
@@ -389,16 +288,12 @@ Module Examples.
     Definition papp_cons {A} (x : A) (xs : list A) := let my_cons := @cons in
                                                       my_cons A x xs.
 
-    MetaCoq Run (eta_expand_def
-                 false false
-                 <%% @papp_cons %%>.1
-                 (only_from_module_of <%% @papp_cons %%>)
-                 papp_cons).
+    MetaCoq Run (eta_expand_def false false papp_cons).
   End Ex4.
 
   Module Ex5.
 
-    (* Mutial inductive *)
+    (* Mutual inductive *)
     Inductive even : nat -> Type :=
     | even_O : even 0
     | even_S : forall n, odd n -> even (S n)
@@ -409,11 +304,7 @@ Module Examples.
       let f := odd_S 0 in
       f even_O.
 
-    MetaCoq Run (eta_expand_def
-                   false false
-                   <%% papp_odd %%>.1
-                   (only_from_module_of <%% papp_odd %%>)
-                   papp_odd).
+    MetaCoq Run (eta_expand_def false false papp_odd).
 
     Inductive Expr (Annot : Type) :=
     | eNat : nat -> Expr Annot
@@ -428,11 +319,125 @@ Module Examples.
       let part_app := eApp _ (eFn unit "f" (eNat unit 0)) in
       part_app (eCons _ (eNat unit 0) (eNil _)).
 
-    MetaCoq Run (eta_expand_def
-                   false false
-                   <%% papp_expr %%>.1
-                   (only_from_module_of <%% papp_expr %%>)
-                   papp_expr).
+    MetaCoq Run (eta_expand_def false false  papp_expr).
   End Ex5.
 
+  Module Ex_branches1.
+    Definition nat_cons (x : nat) (xs : list nat) := x :: xs.
+
+    (** A hand-crafted example with the second branch requiring expansion  *)
+    Definition match_ex1_syn :=
+      (tLambda
+       {|
+       binder_name := nNamed "xs";
+       binder_relevance := Relevant |}
+       (tApp
+          (tInd
+             {|
+             inductive_mind := (MPfile ["Datatypes"; "Init"; "Coq"],
+                               "list");
+             inductive_ind := 0 |} [])
+          [tInd
+             {|
+             inductive_mind := (MPfile ["Datatypes"; "Init"; "Coq"],
+                               "nat");
+             inductive_ind := 0 |} []])
+       (tCase
+          ({|
+           inductive_mind := (MPfile ["Datatypes"; "Init"; "Coq"],
+                             "list");
+           inductive_ind := 0 |}, 1, Relevant)
+          (tLambda
+             {|
+             binder_name := nNamed "xs";
+             binder_relevance := Relevant |}
+             (tApp
+                (tInd
+                   {|
+                   inductive_mind := (MPfile
+                                      ["Datatypes"; "Init"; "Coq"],
+                                     "list");
+                   inductive_ind := 0 |} [])
+                [tInd
+                   {|
+                   inductive_mind := (MPfile
+                                      ["Datatypes"; "Init"; "Coq"],
+                                     "nat");
+                   inductive_ind := 0 |} []])
+             (tApp
+                (tInd
+                   {|
+                   inductive_mind := (MPfile
+                                      ["Datatypes"; "Init"; "Coq"],
+                                     "list");
+                   inductive_ind := 0 |} [])
+                [tInd
+                   {|
+                   inductive_mind := (MPfile
+                                      ["Datatypes"; "Init"; "Coq"],
+                                     "nat");
+                   inductive_ind := 0 |} []]))
+          (tRel 0)
+          [(0,
+           tApp
+             (tConstruct
+                {|
+                inductive_mind := (MPfile
+                                     ["Datatypes"; "Init"; "Coq"],
+                                  "list");
+                inductive_ind := 0 |} 0 [])
+             [tInd
+                {|
+                inductive_mind := (MPfile
+                                     ["Datatypes"; "Init"; "Coq"],
+                                  "nat");
+                inductive_ind := 0 |} []]);
+          (2, tApp
+             (tConstruct
+                {|
+                inductive_mind := (MPfile
+                                     ["Datatypes"; "Init"; "Coq"],
+                                  "list");
+                inductive_ind := 0 |} 1 [])
+             [tInd
+                {|
+                inductive_mind := (MPfile
+                                     ["Datatypes"; "Init"; "Coq"],
+                                  "nat");
+                inductive_ind := 0 |} []])])).
+
+    MetaCoq Unquote Definition match_ex1 := match_ex1_syn.
+
+    MetaCoq Quote Recursively Definition match_ex1__ := match_ex1.
+    MetaCoq Run (eta_expand_def
+     (* We set the trimmig of masks to true, so the procedure does't not perform full expansion.
+        That way we can test the expansion of branches *)
+                   true true
+                   match_ex1).
+
+    MetaCoq Quote Definition match_ex1_expanded_syn := (unfolded ConCert_Extraction_CertifyingEta_Examples_Ex_branches1_match_ex1_expanded).
+
+    (* We just check that they are not syntactically different, nothing more thorough *)
+    Lemma match_ex1_syn_neq_expanded :
+      match_ex1_syn <> match_ex1_expanded_syn.
+    Proof. intro H. inversion H. Qed.
+
+  End Ex_branches1.
+
+  (** An example requiring branch expansion from the standard library *)
+  Module Ex_branches2.
+    Definition anchor := fun x : nat => x.
+    Definition CURRENT_MODULE := Eval compute in <%% anchor %%>.1.
+
+    MetaCoq Quote Definition sig_rect_syn := (unfolded sig_rect).
+
+    MetaCoq Run (eta_expand_def true true sig_rect).
+
+    MetaCoq Quote Definition sig_rect_expanded_syn := (unfolded Coq_Init_Specif_sig_rect_expanded).
+
+    Lemma sig_rec_syn_neq_expanded :
+      sig_rect_syn <> sig_rect_expanded_syn.
+    Proof. intros H. inversion H. Qed.
+
+  End Ex_branches2.
 End Examples.
