extraction/theories/LiquidityExtract.v
@@ -17,7 +17,7 @@ From ConCert.Embedding Require Import Notations.
 From ConCert.Embedding Require Import SimpleBlockchain.
 
 From ConCert.Extraction Require Import LPretty
-     Common ExAst Erasure Optimize Extraction SpecializeChainBase Inlining.
+     Common ExAst Erasure Optimize Extraction CertifyingInlining Certifying SpecializeChainBase.
 
 From Coq Require Import List Ascii String.
 Local Open Scope string_scope.
@@ -50,55 +50,56 @@ Arguments lmd_init_prelude {_ _ _ _ _}.
 Arguments lmd_receive {_ _ _ _ _}.
 Arguments lmd_entry_point {_ _ _ _ _}.
 
+
 (* Extract an environment with some minimal checks. This assumes the environment
    is well-formed (to make it computable from within Coq) but furthermore checks that the
    erased context is closed, expanded and that the masks are valid before dearging.
    Takes [should_inline] - a map that returns true for the constants that should be inlined.
    Suitable for extraction of programs **from within Coq**. *)
-   Definition extract_liquidity_within_coq (should_inline : kername -> bool) :=
-    {| check_wf_env_func Σ := Ok (assume_env_wellformed Σ);
-       pcuic_args :=
-         {| optimize_prop_discr := true;
-            transforms := [dearg_transform true true true true true;
-                           Inlining.transform should_inline ] |} |}.
-  
-  Definition extract (should_inline : kername -> bool)
-    := extract_template_env (extract_liquidity_within_coq should_inline).
+Definition extract_liquidity_within_coq (to_inline : kername -> bool)
+           (seeds : KernameSet.t) :=
+  {| check_wf_env_func Σ := Ok (assume_env_wellformed Σ);
+     template_transforms :=
+       [CertifyingInlining.template_inline to_inline];
+     pcuic_args :=
+       {| optimize_prop_discr := true;
+          extract_transforms :=
+            [dearg_transform true true true true true ] |} |}.
 
-(* Machinery for specializing chain base *)
-Definition extract_template_env_specialize
-           (should_inline : kername -> bool)
-           (params : extract_template_env_params)
-           (Σ : global_env)
+Definition extract (to_inline :  kername -> bool)
            (seeds : KernameSet.t)
-           (ignore : kername -> bool) : result ExAst.global_env string :=
-  let Σ := SafeTemplateChecker.fix_global_env_universes Σ in
-  let Σ := TemplateToPCUIC.trans_global_decls Σ in
-  Σ <- specialize_ChainBase_env Σ ;;
-  wfΣ <- check_wf_env_func params Σ;;
-  extract_pcuic_env (pcuic_args params) Σ wfΣ seeds ignore.
+           (extract_ignore : kername -> bool)
+           (Σ : global_env) : TemplateMonad ExAst.global_env
+  := extract_template_env_certifying_passes ret (extract_liquidity_within_coq to_inline seeds) Σ seeds extract_ignore.
 
-Definition extract_template_env_within_coq_specialize inline := extract_template_env_specialize inline (extract_liquidity_within_coq inline).
 
-Definition printLiquidityDefs_ 
-           (extract_template_env : (kername -> bool) -> global_env -> KernameSet.t -> (kername -> bool) -> result ExAst.global_env string)
+Definition extract_specialize (to_inline :  kername -> bool)
+           (seeds : KernameSet.t)
+           (extract_ignore : kername -> bool)
+           (Σ : global_env) : TemplateMonad ExAst.global_env
+  := extract_template_env_certifying_passes specialize_ChainBase_env (extract_liquidity_within_coq to_inline seeds) Σ seeds extract_ignore.
+
+Definition printLiquidityDefs_
+           (extract_env : (kername -> bool) -> KernameSet.t -> (kername -> bool) -> global_env -> TemplateMonad ExAst.global_env)
            (prefix : string) (Σ : global_env)
            (TT : MyEnv.env string)
-           (ignore : list kername)
            (inline : list kername)
+           (ignore : list kername)
            (build_call_ctx : string)
            (init_prelude : string)
            (init : kername)
            (receive : kername)
-  : string + string :=
+
+  : TemplateMonad string :=
   let seeds := KernameSet.union (KernameSet.singleton init) (KernameSet.singleton receive) in
-  match extract_template_env (fun k => List.existsb (eq_kername k) inline) Σ seeds (fun k => List.existsb (eq_kername k) ignore) with
-  | Ok eΣ =>
-    (* dependencies should be printed before the dependent definitions *)
-    let ldef_list := List.rev (print_global_env prefix TT eΣ) in
-    (* filtering empty strings corresponding to the ignored definitions *)
-    let ldef_list := filter (negb ∘ (String.eqb "") ∘ snd) ldef_list in
-    match ExAst.lookup_env eΣ init with
+  let should_inline kn := existsb (eq_kername kn) inline in
+  let ignore_extract kn := List.existsb (eq_kername kn) ignore in
+  eΣ <- extract_env should_inline seeds ignore_extract Σ ;;
+  (* dependencies should be printed before the dependent definitions *)
+  let ldef_list := List.rev (print_global_env prefix TT eΣ) in
+  (* filtering empty strings corresponding to the ignored definitions *)
+  let ldef_list := filter (negb ∘ (String.eqb "") ∘ snd) ldef_list in
+  match ExAst.lookup_env eΣ init with
     | Some (ExAst.ConstantDecl init_cst) =>
       match print_init prefix TT build_call_ctx init_prelude eΣ init_cst with
       | Some init_code =>
@@ -107,19 +108,17 @@ Definition printLiquidityDefs_
             map snd (filter (negb ∘ (eq_kername init) ∘ fst) ldef_list) in
         let res :=
             concat (nl ++ nl) (defs ++[ init_code ]) %list in
-        inl res
-      | None => inr "Error: Empty body for init"
+        ret res
+      | None => tmFail "Error: Empty body for init"
       end
-    | Some _ => inr "Error: init must be a constant"
-    | None => inr "Error: No init found"
-    end
-  | Err e => inr e
+    | Some _ => tmFail "Error: init must be a constant"
+    | None => tmFail "Error: No init found"
   end.
 
 (* standard printing of definitions *without* chainbase specialization *)
 Definition printLiquidityDefs := printLiquidityDefs_ extract.
 (* printing *with* chainbase specialization *)
-Definition printLiquidityDefs_specialize := printLiquidityDefs_ extract_template_env_within_coq_specialize.
+Definition printLiquidityDefs_specialize := printLiquidityDefs_ extract_specialize.
 
 
 Definition liquidity_ignore_default :=
@@ -199,14 +198,15 @@ Definition liquidity_call_ctx :=
 
 Definition liquidity_extract_args :=
   {| check_wf_env_func := check_wf_env_func extract_within_coq;
+     template_transforms := [];
      pcuic_args :=
        {| optimize_prop_discr := true;
-          transforms := [dearg_transform
-                           true
-                           false (* cannot have partially applied ctors *)
-                           true
-                           true
-                           true] |} |}.
+          extract_transforms := [dearg_transform
+                                 true
+                                 false (* cannot have partially applied ctors *)
+                                 true
+                                 true
+                                 true] |} |}.
 
 Definition liquidity_simple_extract
            (TT_defs : list (kername *  string))
@@ -236,12 +236,12 @@ Definition wrap_in_delimiters s :=
   String.concat nl ["";"(*START*)"; s; "(*END*)"].
 
 Definition liquidity_extraction_ {msg ctx params storage operation : Type}
-           (printLiquidityDefs_ : string ->
+           (printLiquidityDefs : string ->
                                  global_env ->
                                  env string ->
                                  list kername ->
                                  list kername ->
-                                 string -> string -> kername -> kername -> string + string)
+                                 string -> string -> kername -> kername -> TemplateMonad string)
            (prefix : string)
            (TT_defs : list (kername *  string))
            (TT_ctors : MyEnv.env string)
@@ -253,17 +253,12 @@ Definition liquidity_extraction_ {msg ctx params storage operation : Type}
   let ignore := (map fst TT_defs ++ liquidity_ignore_default)%list in
   let TT :=
       (TT_ctors ++ map (fun '(kn,d) => (string_of_kername kn, d)) TT_defs)%list in
-  p <- tmEval lazy
-             (printLiquidityDefs_ prefix Σ TT ignore inline
-                                 liquidity_call_ctx
-                                 m.(lmd_init_prelude)
-                                 init_nm receive_nm) ;;
-  match p with
-  | inl s =>
+  s <- printLiquidityDefs prefix Σ TT inline ignore
+                         liquidity_call_ctx
+                         m.(lmd_init_prelude)
+                             init_nm receive_nm ;;
     tmEval lazy
-           (wrap_in_delimiters (concat (nl ++ nl) [m.(lmd_prelude); s; m.(lmd_entry_point)]))
-  | inr s => tmFail s
-  end.
+           (wrap_in_delimiters (concat (nl ++ nl) [m.(lmd_prelude); s; m.(lmd_entry_point)])).
 
 (* Liquidity extraction *without* chainbase specialization *)
 Definition liquidity_extraction {msg ctx params storage operation : Type} := @liquidity_extraction_ msg ctx params storage operation printLiquidityDefs.
